Some work on term and fol

src/coq/coqprover/procedure.v
@@ -1,48 +1,60 @@
-Require Import logic.
+Require Import logic .
 Require Import List .
-
-(* paths -> Coinductive lists?*)
-
-(* Parameter Path : Set .*)
+Require Import Arith .
 
 Definition Path := nat -> option Model.
 
-
-(*
 Definition PathTo (tau : Path) (n : nat) : Path :=
-  fun i : nat => if (i > n) then None
-           else tau i . 
-*)
-Parameter PathTo : Path -> nat -> Path .
-Parameter PathFrom : Path -> nat -> Path .
-Parameter nth : Path -> nat -> Model .
+  fun (i : nat) => if (leb n i)
+                   then None
+                   else tau i . 
 
-(* TODO: prefix? -> needed for def of complete execution paths *)
+
+Definition PathFrom (tau : Path) (n : nat) : Path :=
+  fun (i : nat) => if (leb i n)
+                   then tau i
+                   else None .
+
+Definition nth (tau : Path) (n : nat) : option Model := tau n.
+
+
 Parameter Path_eq_dec : Path -> Path -> Prop .
 Definition isPrefix (p : Path) (P : Path) := exists i, Path_eq_dec (PathTo P i) p .
 
-(* proper prefix! *)
-Definition complete (P : Path) := forall p : Path, not (isPrefix P p) .
+Definition isProperPrefix (p : Path) (P : Path) := exists i, (Path_eq_dec (PathTo P i) p /\ not (nth P (i + 1) = None)) .
+
+Lemma prefix: forall p, forall P, isProperPrefix p P -> isPrefix p P .
+Proof.
+  intros.
+  destruct H.
+  destruct H.
+  unfold isPrefix.
+  exists x.
+  assumption.
+Qed.  
+
+Definition completePath (P : Path) := forall p : Path, not (isProperPrefix P p) .
 
 Definition StartsFrom (tau : Path) (rho : Valuation) (phi : MLFormula) :=
-  Satisfies (nth tau 0) rho phi .
+  exists gamma, nth tau 0 = Some gamma /\ Satisfies gamma rho phi .
 
 
 (* All Paths Reachability Satisfaction *)
 
-Inductive APRLFormula := rl : MLFormula -> MLFormula -> APRLFormula .
-Notation "L ==> R" := (rl L R) (at level 100).
-Fixpoint Lhs (r : APRLFormula) := match r with (L ==> _) => L end . 
-Fixpoint Rhs (r : APRLFormula) := match r with (_ ==> R) => R end . 
+Definition APRLFormula := (MLFormula*MLFormula)%type .
+Notation "L ==> R" := (L, R) (at level 100).
+Notation Lhs := fst.
+Notation Rhs := snd. 
 
 Parameter isInfinite : Path -> Prop .
-Parameter infiniteIsComplete : forall p : Path, isInfinite p -> complete p .
+Parameter infiniteIsComplete : forall p : Path, isInfinite p -> completePath p .
 
 
 (* (tau, rho) |= phi ==> phi' *)
 Definition entails (tau : Path) (rho : Valuation) (F : APRLFormula) :=
   (StartsFrom tau rho (Lhs F)) ->
-  (or (exists i, Satisfies (nth tau i) rho (Rhs F))
+  (or (exists i, exists gamma,
+                   (nth tau i = Some gamma) /\ Satisfies gamma rho (Rhs F))
       (isInfinite tau)).
 
 (* =>S |= phi ==> phi' *)
@@ -50,10 +62,20 @@ Definition entailsTS (TS : RLSystem -> Model -> Model -> Prop) (F : APRLFormula)
   := forall (tau : Path), forall (rho : Valuation),
        (StartsFrom tau rho (Lhs F)) -> (entails tau rho F) .
 
+(*
+Definition f : { x : nat | x > 5 } -> nat := fun n => n-1.
+Lemma f_prop : forall n, f n > 4
+
+Definition f' : nat -> nat := x-1.
+Lemma f'_prop : forall n, n > 5 -> f n > 4
+                                 
+Definition pos := nat.
 
 (* Semantics for phi ==> phi' *)
 Definition sem (F: APRLFormula) :=
   { tau : Path & (exists (rho : Valuation), entails tau rho F) } .
+*)
+
 
 
 (* S-Derivative *)
@@ -63,18 +85,100 @@ Definition SDerivative (phi phi' phi1 : MLFormula) :=
     (exists (tau : Path),
        entails tau rho (phi ==> phi') /\ (Path_eq_dec tau1 (PathFrom tau 1))).
 
-(* Proper S-Derivative *)
+(* Proper S-Derivative  phi1 => phi'  phi => phi' *)
 Definition ProperSDerivative (phi phi' phi1 : MLFormula) :=
-  SDerivative phi phi' phi1 /\ not (Empty_set = sem (phi ==> phi')).
+  SDerivative phi phi' phi1 /\
+  (exists tau, exists rho, entails tau rho (phi ==> phi')) .
 
 (* S-Derivable *)
 Definition SDerivable (F : APRLFormula) :=
   exists (phi1 : MLFormula), ProperSDerivative (Lhs F) (Rhs F) phi1 .
 
 (* Complete *)
-(*
-Definition complete (Delta : Set) := 
- *)
+Definition completeSetsOfDer (Δ : list APRLFormula) (phi phi' : MLFormula):=
+  forall (phi1 : MLFormula),
+    SDerivative phi phi' phi1 -> In (phi1 ==> phi') Δ.
+                             
+      
 
 (* FOL encoding *)
-Definition fol (phi : MLFormula) := 
+Fixpoint bp (phi : MLFormula) : list MLFormula :=
+  match phi with
+    | T => nil
+    | Bp C => (Bp C) :: nil
+    | Fol F => nil
+    | Not phi' => bp phi'
+    | And phi' phi'' => (bp phi') ++ (bp phi'') 
+    | Or phi' phi'' => (bp phi') ++ (bp phi'') 
+    | Implies phi' phi'' => (bp phi') ++ (bp phi'') 
+    | logic.Exists v phi' => (bp phi')
+  end.
+
+Fixpoint conjGen (L : list MLFormula) : MLFormula :=
+  match L with
+    | t :: nil => ??
+    | C :: Rest => Equals C (conjGen Rest)
+  end.
+
+Fixpoint phiEQ (phi : MLFormula) (conj : MLFormula) : MLFormula :=
+  match phi with
+    | T => T
+    | Bp C => conj
+    | Not phi' => phiEQ phi' conj
+    | And phi' phi'' => And (phiEQ phi' conj) (phiEQ phi'' conj) 
+    | Or phi' phi'' => Or (phiEQ phi' conj) (phiEQ phi'' conj) 
+    | Implies phi' phi'' => Implies (phiEQ phi' conj) (phiEQ phi'' conj) 
+    | logic.Exists v phi' => logic.Exists v (phiEQ phi' conj)
+    | Equals phi' phi'' => Equals (phiEQ phi' conj) (phiEQ phi'' conj)
+  end.
+
+
+
+Parameter pi1 : logic.Cfg.
+Parameter pi2 : logic.Cfg.
+Parameter pi3 : logic.Cfg.
+Parameter pi4 : logic.Cfg.
+
+(* (pi1 /\ T) /\ ( pi2 -> not pi3  \/ pi4 ) *)
+Eval compute in
+    And
+      (And (Bp pi1) T)
+      (Or
+         (Implies (Bp pi2) (Not (Bp pi3)))
+         (Bp pi4)
+      ).
+
+Eval compute in bp (And
+      (And (Bp pi1) T)
+      (Or
+         (Implies (Bp pi2) (Not (Bp pi3)))
+         (Bp pi4)
+      ))
+.
+
+Eval compute in conjGen (bp (And
+      (And (Bp pi1) T)
+      (Or
+         (Implies (Bp pi2) (Not (Bp pi3)))
+         (Bp pi4)
+      ))).
+
+Eval compute in phiEQ
+                  (And
+                     (And (Bp pi1) T)
+                     (Or
+                        (Implies (Bp pi2) (Not (Bp pi3)))
+                        (Bp pi4)
+                     ))
+                  (conjGen (bp (And
+      (And (Bp pi1) T)
+      (Or
+         (Implies (Bp pi2) (Not (Bp pi3)))
+         (Bp pi4)
+      )))).
+
+
+Definition phi := Or (And (Bp pi1) T) (And (Bp pi2) T).
+Eval compute in phi .
+Eval compute in bp phi.
+Eval compute in conjGen (bp phi) .
