src/coq/coqprover/fol.v
@@ -1,0 +1,46 @@
+Require Import term.
+Require Import List.
+
+Parameter PSymbol : Set .
+Definition Predicates := list (PSymbol * list Sort)%type .
+
+Parameter Σ : Signature .
+Parameter Π : Predicates .
+
+Definition FOLSignature := (Σ, Π).
+
+
+Inductive FOLFormula :=
+| t : FOLFormula
+| pred : PSymbol -> list Term -> FOLFormula
+| notFOL : FOLFormula -> FOLFormula
+| andFOL : FOLFormula -> FOLFormula -> FOLFormula
+| existsFOL : list Var -> FOLFormula -> FOLFormula .
+
+(* TODO 
+Fixpoint wff (Φ : FOLSignature) (f : FOLFormula) :=
+*)
+
+
+
+
+
+
+
+Variables p1 p2 : PSymbol.
+Variables f1 f2 : OpSymbol .
+Variables s1 s2 : Sort.
+Variables v1 v2 : Var .
+
+Definition Sigma := sig (s1 :: s2 :: nil)
+                        ((f1, ((s1 :: s1 :: nil), s2)) ::
+                        (f2, ((s1 :: nil), s1)) :: nil) .
+
+Definition Pi := (p1, (s1 :: s2 ::nil)) :: nil .
+
+Definition S := (Sigma, Pi) .
+
+Eval compute in tcst f1 .
+Eval compute in tvar v1.
+Eval compute in (p1, s1 :: s1 :: nil) :: nil .
+Eval compute in pred p1 ((tcst f1) :: (tvar v1) :: nil) . 
