src/coq/coqprover/logic.v
@@ -1,24 +1,22 @@
+Require Import term.
+Require Import fol.
 
-Parameter Var : Set .
 
-Parameter CfgTerm : Set .
+Parameter Cfg : Type .
 
-Parameter VarToTerm : Var -> Term.
-
-Coercion VarToTerm : Var >-> Term.
-
+Parameter CfgToTerm : Cfg -> Term .
+Coercion CfgToTerm : Cfg >-> Term .
 
 (* helpers *)
 Parameter isVariable : Term -> Prop .
-
-(* Variables *)
-(* Definition Var := { x : Term & (isVariable x) }. *)
+Parameter Cfg_eq_dec : Cfg -> Cfg -> Prop .
 
 
 (* Matching Logic Formulas = MLFormula *)
 Inductive MLFormula :=
   | T : MLFormula
-  | Bp : Term -> MLFormula
+  | Bp : Cfg -> MLFormula
+  | Fol : FOLFormula -> MLFormula 
   | Not : MLFormula -> MLFormula
   | And : MLFormula -> MLFormula -> MLFormula
   | Or : MLFormula -> MLFormula -> MLFormula
@@ -27,8 +25,8 @@ Inductive MLFormula :=
 .
 
 (* Model and Valuation *)
-Parameter Model : Set .
-Parameter Valuation : Set (* Var -> Model *) .
+Parameter Model : Type .
+Parameter Valuation : Type (* Var -> Model *) .
 
 
 (* Satisfaction relation*)
@@ -38,12 +36,13 @@ Parameter Satisfies : Model -> Valuation -> MLFormula -> Prop .
 (* Reachability Logic Formulas = RLFormula *)
 
 Definition RLFormula := (MLFormula * MLFormula)%type .
-
 Notation "L => R" := (L, R) (at level 100).
+Notation lhs := fst.
+Notation rhs := snd.
 
 Definition RLSystem := RLFormula -> Prop .
 
 (* Transition system *)
 Definition TS (S : RLSystem) (gamma : Model) (gamma' : Model) :=
   exists F : RLFormula, exists rho : Valuation,
-                          (S F /\ Satisfies gamma rho (fst F) /\ Satisfies gamma' rho (snd F)).
+                          (S F /\ Satisfies gamma rho (lhs F) /\ Satisfies gamma' rho (rhs F)).
