src/coq/coqprover/term.v
@@ -1,0 +1,74 @@
+Require Import List .
+Require Import String .
+Require Import ZArith.
+
+Parameter Sort : Type .
+Parameter OpSymbol : Type . (* QIds as in Maude? *)
+Parameter Var : Type .
+
+(* Many-sorted signature *)
+Record Signature :=
+  sig {
+      sorts : list Sort; (* really needed? *)
+      ops : list (OpSymbol * ((list Sort) * Sort))
+    } .
+
+(* Terms *)
+Inductive Term : Type :=
+| tcst : OpSymbol -> Term
+| tvar : Var -> Term
+| tcom : OpSymbol -> list Term -> Term .
+
+
+(* TODO: Well-formed sigma terms *)
+(*
+Fixpoint wf (Σ : Signature) (t : Term) : bool := TODO
+*)
+
+(*
+Variables a b c : Sort .
+Variables s t : OpSymbol .
+Eval compute in sig (a :: b :: nil)
+                    ((s, ((a :: c :: nil), b)) ::
+                    (t, ((a :: nil), c)) :: nil) .
+Definition S := sig (a :: b :: nil)
+                    ((s, ((a :: c :: nil), b)) ::
+                                               (t, ((a :: nil), c)) :: nil) .
+
+Eval compute in ops S .
+
+(*
+
+Inductive AExp :=
+| int : Z -> AExp
+| id : string -> AExp
+| add : AExp -> AExp -> AExp .
+
+Inductive BExp :=
+| bl : bool -> BExp
+| less : AExp -> AExp -> BExp 
+| and : BExp -> BExp -> BExp 
+| not : BExp -> BExp .
+
+Inductive Stmt :=
+| skip : Stmt
+| ifStmt : BExp -> Stmt -> Stmt -> Stmt
+| while : BExp -> Stmt -> Stmt
+| stmts : Stmt -> Stmt -> Stmt .
+
+
+
+(* Semantics of sorts and operations *)
+Parameter sortSem : list Sort -> Type .
+Parameter opsSem : list (Symbol * ((list Sort) * Sort)) -> Type .
+
+(* ΣAlgebra *)
+Record ΣAlgebra (sigma : Signature) : Type :=
+  alg {
+      carrierSets : (sortSem (sorts sigma));
+      functions : (opsSem (operations sigma))
+    } .
+
+
+
+*)*)
